\begin{prooftree}
\AxiomC{$A \rightarrow A$}
\RightLabel{[$\neg$L]}
\UnaryInfC{$\neg A, A \rightarrow $}
\RightLabel{[$\land$L]}
\UnaryInfC{$(\neg A \land \neg B), A \rightarrow $}
\RightLabel{[$\neg$R]}
\UnaryInfC{$A \rightarrow \neg (\neg A \land \neg B)$}
\AxiomC{$B \rightarrow B$}
\RightLabel{[$\neg$L]}
\UnaryInfC{$\neg B, B \rightarrow $}
\RightLabel{[$\land$L]}
\UnaryInfC{$(\neg A \land \neg B), B \rightarrow $}
\RightLabel{[$\neg$R]}
\UnaryInfC{$B \rightarrow \neg (\neg A \land \neg B)$}
\RightLabel{[$\lor$L]}
\BinaryInfC{$(A \lor B) \rightarrow \neg (\neg A \land \neg B)$}
\RightLabel{[$\supset$R]}
\UnaryInfC{$ \rightarrow ((A \lor B) \supset \neg (\neg A \land \neg B))$}
\AxiomC{$A \rightarrow A$}
\RightLabel{[$\lor$R]}
\UnaryInfC{$A \rightarrow (A \lor B)$}
\RightLabel{[$\neg$R]}
\UnaryInfC{$ \rightarrow (A \lor B), \neg A$}
\AxiomC{$B \rightarrow B$}
\RightLabel{[$\lor$R]}
\UnaryInfC{$B \rightarrow (A \lor B)$}
\RightLabel{[$\neg$R]}
\UnaryInfC{$ \rightarrow (A \lor B), \neg B$}
\RightLabel{[$\land$R]}
\BinaryInfC{$ \rightarrow (A \lor B), (\neg A \land \neg B)$}
\RightLabel{[$\neg$L]}
\UnaryInfC{$\neg (\neg A \land \neg B) \rightarrow (A \lor B)$}
\RightLabel{[$\supset$R]}
\UnaryInfC{$ \rightarrow (\neg (\neg A \land \neg B) \supset (A \lor B))$}
\RightLabel{[$\land$R]}
\BinaryInfC{$ \rightarrow ((A \lor B) \equiv \neg (\neg A \land \neg B))$}
\end{prooftree}
