\begin{prooftree}
\AxiomC{$A \rightarrow A$}
\RightLabel{[$\neg$R]}
\UnaryInfC{$ \rightarrow A, \neg A$}
\RightLabel{[$\lor$R]}
\UnaryInfC{$ \rightarrow A, (\neg A \lor \neg B)$}
\RightLabel{[XR]}
\UnaryInfC{$ \rightarrow (\neg A \lor \neg B), A$}
\AxiomC{$B \rightarrow B$}
\RightLabel{[$\neg$R]}
\UnaryInfC{$ \rightarrow B, \neg B$}
\RightLabel{[$\lor$R]}
\UnaryInfC{$ \rightarrow B, (\neg A \lor \neg B)$}
\RightLabel{[XR]}
\UnaryInfC{$ \rightarrow (\neg A \lor \neg B), B$}
\RightLabel{[$\land$R]}
\BinaryInfC{$ \rightarrow (\neg A \lor \neg B), (A \land B)$}
\RightLabel{[$\neg$L]}
\UnaryInfC{$\neg (A \land B) \rightarrow (\neg A \lor \neg B)$}
\RightLabel{[$\supset$R]}
\UnaryInfC{$ \rightarrow (\neg (A \land B) \supset (\neg A \lor \neg B))$}
\AxiomC{$A \rightarrow A$}
\RightLabel{[$\land$L]}
\UnaryInfC{$(A \land B) \rightarrow A$}
\RightLabel{[$\neg$R]}
\UnaryInfC{$ \rightarrow A, \neg (A \land B)$}
\RightLabel{[XR]}
\UnaryInfC{$ \rightarrow \neg (A \land B), A$}
\RightLabel{[$\neg$L]}
\UnaryInfC{$\neg A \rightarrow \neg (A \land B)$}
\AxiomC{$B \rightarrow B$}
\RightLabel{[$\land$L]}
\UnaryInfC{$(A \land B) \rightarrow B$}
\RightLabel{[$\neg$R]}
\UnaryInfC{$ \rightarrow B, \neg (A \land B)$}
\RightLabel{[XR]}
\UnaryInfC{$ \rightarrow \neg (A \land B), B$}
\RightLabel{[$\neg$L]}
\UnaryInfC{$\neg B \rightarrow \neg (A \land B)$}
\RightLabel{[$\lor$L]}
\BinaryInfC{$(\neg A \lor \neg B) \rightarrow \neg (A \land B)$}
\RightLabel{[$\supset$R]}
\UnaryInfC{$ \rightarrow ((\neg A \lor \neg B) \supset \neg (A \land B))$}
\RightLabel{[$\land$R]}
\BinaryInfC{$ \rightarrow (\neg (A \land B) \equiv (\neg A \lor \neg B))$}
\end{prooftree}
