\begin{prooftree}
\AxiomC{$F(a) \rightarrow F(a)$}
\RightLabel{[$\land$L]}
\UnaryInfC{$(F(a) \land G(a)) \rightarrow F(a)$}
\RightLabel{[$\forall$L]}
\UnaryInfC{$\forall x (F(x) \land G(x)) \rightarrow F(a)$}
\RightLabel{[$\forall$R]}
\UnaryInfC{$\forall x (F(x) \land G(x)) \rightarrow \forall x F(x)$}
\AxiomC{$G(a) \rightarrow G(a)$}
\RightLabel{[$\land$L]}
\UnaryInfC{$(F(a) \land G(a)) \rightarrow G(a)$}
\RightLabel{[$\forall$L]}
\UnaryInfC{$\forall x (F(x) \land G(x)) \rightarrow G(a)$}
\RightLabel{[$\forall$R]}
\UnaryInfC{$\forall x (F(x) \land G(x)) \rightarrow \forall x G(x)$}
\RightLabel{[$\land$R]}
\BinaryInfC{$\forall x (F(x) \land G(x)) \rightarrow (\forall x F(x) \land \forall x G(x))$}
\RightLabel{[$\supset$R]}
\UnaryInfC{$ \rightarrow (\forall x (F(x) \land G(x)) \supset (\forall x F(x) \land \forall x G(x)))$}
\AxiomC{$F(a) \rightarrow F(a)$}
\RightLabel{[$\forall$L]}
\UnaryInfC{$\forall x F(x) \rightarrow F(a)$}
\RightLabel{[$\land$L]}
\UnaryInfC{$(\forall x F(x) \land \forall x G(x)) \rightarrow F(a)$}
\AxiomC{$G(a) \rightarrow G(a)$}
\RightLabel{[$\forall$L]}
\UnaryInfC{$\forall x G(x) \rightarrow G(a)$}
\RightLabel{[$\land$L]}
\UnaryInfC{$(\forall x F(x) \land \forall x G(x)) \rightarrow G(a)$}
\RightLabel{[$\land$R]}
\BinaryInfC{$(\forall x F(x) \land \forall x G(x)) \rightarrow (F(a) \land G(a))$}
\RightLabel{[$\forall$R]}
\UnaryInfC{$(\forall x F(x) \land \forall x G(x)) \rightarrow \forall x (F(x) \land G(x))$}
\RightLabel{[$\supset$R]}
\UnaryInfC{$ \rightarrow ((\forall x F(x) \land \forall x G(x)) \supset \forall x (F(x) \land G(x)))$}
\RightLabel{[$\land$R]}
\BinaryInfC{$ \rightarrow (\forall x (F(x) \land G(x)) \equiv (\forall x F(x) \land \forall x G(x)))$}
\end{prooftree}
